progress on lc_join_path_split

Disjoint.v
@@ -27,49 +27,94 @@ Module Disjoint.
   Definition DisjointBranch `{redCFG} (s : Lab) (xl : list Var) (qt qf : Lab) (π ϕ : list Lab) :=
     CPath s qt (π >: s) /\ CPath s qf (ϕ >: s) /\ branch s =' xl /\ Disjoint π ϕ.
 
-  Parameter path_splits : forall `{redCFG}, Lab -> list (Lab * Lab * Lab * list Var).
+  Parameter path_splits : forall `{redCFG}, Lab -> list (Lab * Lab * Lab).
 
-  Parameter loop_splits : forall `{redCFG}, Lab -> Lab -> list (Lab * Lab * Lab * list Var).
+  Parameter loop_splits : forall `{redCFG}, Lab -> Lab -> list (Lab * Lab * Lab).
 
-  Definition pl_split `{redCFG} (qh qe q1 q2 br : Lab) (xl : list Var) :=
+  (* remove branch from splits, we can use the assumed global branch function to get varsets back*)
+  Definition pl_split `{redCFG} (qh qe q1 q2 br : Lab) :=
       (exists π ϕ, CPath br qh (π >: q1 :>: br)
               /\ CPath br qe (ϕ >: q2 :>: br)
-              /\ Disjoint (tl π :r: q1) (tl ϕ :r: q2) 
-              /\ branch br =' xl).
+              /\ Disjoint (tl π :r: q1) (tl ϕ :r: q2)).
 
-  Parameter path_splits_spec : forall `{redCFG} p q1 q2 br xl,
-      pl_split p p q1 q2 br xl <->
-      (br, q1, q2, xl) ∈ path_splits p.
+  Parameter path_splits_spec : forall `{redCFG} p q1 q2 br,
+      pl_split p p q1 q2 br <->
+      (br, q1, q2) ∈ path_splits p.
   
-  Parameter loop_splits_spec : forall `{redCFG} qh qe q1 q2 br xl,
+  Parameter loop_splits_spec : forall `{redCFG} qh qe q1 q2 br,
       loop_contains qh br /\ (* otherwise some splits would be considered as loop splits *)
-      pl_split qh qe q1 q2 br xl <->
-      (br, q1, q2, xl) ∈ loop_splits qh qe.  
+      pl_split qh qe q1 q2 br <->
+      (br, q1, q2) ∈ loop_splits qh qe.
 
-  Parameter splits' : forall `{redCFG}, Lab -> Lab -> list (Lab * Lab * Lab * list Var).
-  Parameter splits  : forall `{redCFG}, Lab -> list (Lab * Lab * Lab * list Var).
+  Parameter splits' : forall `{redCFG}, Lab -> Lab -> list (Lab * Lab * Lab).
+  Parameter splits  : forall `{redCFG}, Lab -> list (Lab * Lab * Lab).
 
-  Definition path_splits__imp `{C : redCFG} := @path_splits _ _ _ (implode_CFG C).
-  Definition loop_splits__imp `{C : redCFG} := @loop_splits _ _ _ (implode_CFG C).
+  Definition path_splits__imp `{C : redCFG} p
+    := @path_splits _ _ _ _ (local_impl_CFG C (get_innermost_loop p)) p.
+  Definition loop_splits__imp `{C : redCFG} h
+    := @loop_splits _ _ _ _ (local_impl_CFG C h) h.
 
-  Definition splits'_spec `{redCFG} := forall h e sp, sp ∈ splits' h e
-                                                 <-> sp ∈ loop_splits__imp h e
-                                                   \/ exists br q q' xl, (br,q,q',xl) ∈ loop_splits__imp h e
-                                                                   /\ (sp ∈ splits' br q
-                                                                      \/ sp ∈ splits' br q').
+  Definition splits'_spec `{redCFG} {h': Lab} {H : loop_head h'}
+    := forall h e sp, sp ∈ splits' h e
+                 <-> sp ∈ loop_splits__imp h e
+                   \/ exists br q q', (br,q,q') ∈ loop_splits__imp h e
+                                   /\ (sp ∈ splits' br q
+                                      \/ sp ∈ splits' br q').
 
   Definition splits_spec `{redCFG} := forall p sp, sp ∈ splits p
                                               <-> sp ∈ path_splits__imp p
-                                                \/ exists br q q' xl, (br,q,q',xl) ∈ path_splits__imp p
+                                                \/ exists br q q', (br,q,q') ∈ path_splits__imp p
                                                                 /\ (sp ∈ splits' br q
                                                                    \/ sp ∈ splits' br q').
+
+  Ltac path_simpl' H :=
+    lazymatch type of H with
+    | Path ?edge ?x ?y (?z :<: ?π) => let Q := fresh "Q" in
+                                     eapply path_front in H as Q;
+                                     cbn in Q; subst z
+    | Path ?edge ?x ?y (?π :>: ?z) => let Q := fresh "Q" in
+                                     eapply path_back in H as Q;
+                                     cbn in Q; subst z
+    end.
   
-  Lemma lc_join_path_split `{redCFG} t1 t2 (p q1 q2 s : Lab) (i j1 j2 : Tag)
+  Theorem lc_join_path_split `{redCFG} t1 t2 (p q1 q2 s : Lab) (i : Tag)
         (Hlc : last_common t1 t2 (s,i))
-        (Hneq : q1 <> q2 \/ j1 <> j2)
-        (Hpath1 : TPath' ((p,i) :<: (q1,j1) :< t1))
-        (Hpath2 : TPath' ((p,i) :<: (q2,j2) :< t2))
-    : exists qq qq' xl, (s,qq,qq',xl) ∈ path_splits p.
+        (Hneq : q1 <> q2)
+        (Hpath1 : TPath' ((p,i) :<: (q1,i) :<: t1))
+        (Hpath2 : TPath' ((p,i) :<: (q2,i) :<: t2))
+    : exists qq qq', (s,qq,qq') ∈ path_splits p.
+  Proof.
+    setoid_rewrite <-path_splits_spec. unfold pl_split.
+    unfold TPath' in *;cbn in *. unfold last_common in Hlc; destructH.
+    eapply postfix_path in Hpath1;eauto.
+    2: eapply postfix_cons in Hlc0; eapply postfix_cons in Hlc0;
+      do 2 rewrite <-cons_rcons_assoc in Hlc0; simpl_nl; eassumption.
+    eapply postfix_path in Hpath2;eauto.
+    2: eapply postfix_cons in Hlc2; eapply postfix_cons in Hlc2;
+      do 2 rewrite <-cons_rcons_assoc in Hlc2; simpl_nl; eassumption.
+    assert (forall L ed x y z l, @Path L ed x y (y :<: z :<: l >: x)
+                            -> exists w l', Path ed x y ((l' >: w) :>: x)
+                                      /\ (w :: tl l') ⊆ (z :: l)) as Hppath.
+    {
+      clear. intros. revert dependent y. revert z.
+      induction l; intros z y H;cbn in *.
+      - exists z, (y :: nil). cbn. split;[eassumption|]. firstorder.
+      - inversion H;subst. path_simpl' H1.
+        edestruct IHl as [w [l' IHl']];eauto.
+        exists w, (y :: l'). cbn. unfold ne_rcons in IHl'. split;destructH;[econstructor;eauto|].
+        admit.
+    }
+    eapply TPath_CPath in Hpath1. eapply TPath_CPath in Hpath2. cbn in Hpath2,Hpath1.
+    Lemma ne_map_nl_rcons {A B : Type} (l : list A) a (f : A -> B)
+      : ne_map f (l >: a) = (map f l) >: (f a).
+    Admitted.
+    rewrite ne_map_nl_rcons in Hpath1, Hpath2. cbn in *.
+    eapply Hppath in Hpath1;eauto. eapply Hppath in Hpath2;eauto.
+    destructH. destructH.
+    exists w, w0, l', l'0.
+    split_conj;eauto.
+    (* open : what about q1 ∈ l2' & q2 ∈ l1' ? *)
+    (* /\ move the q1/q2 into the last_common *)
   Admitted.
 
   Definition lc_disj_exit_lsplits_def (d : nat)
@@ -82,7 +127,7 @@ Module Disjoint.
          (Hexit : exited h e)
          (Hpath1 : TPath (ne_back t1) (e,i1) ((e,i1) :<: t1))
          (Hpath2 : TPath (ne_back t2) (e,i2) ((e,i2) :<: t2)),
-      exists (qq qq' : Lab) (xl : list Var), (s,qq,qq',xl) ∈ loop_splits h e.
+      exists (qq qq' : Lab) (xl : list Var), (s,qq,qq') ∈ loop_splits h e.
 
   Definition lc_disj_exits_lsplits_def (d : nat)
     := forall `{redCFG} (s e1 e2 q1 q2 h : Lab) (i1 i2 j k : Tag) t1 t2 (n m : nat)
@@ -98,7 +143,7 @@ Module Disjoint.
          (Hexit2 : exited h e2)
          (Hpath1 : TPath (ne_back t1) (e1,i1) ((e1,i1) :<: t1))
          (Hpath2 : TPath (ne_back t2) (e2,i2) ((e2,i2) :<: t2)),
-      exists (qq qq' : Lab) (xl : list Var), (s,qq,qq',xl) ∈ (loop_splits h e1 ++ loop_splits h e2).
+      exists (qq qq' : Lab), (s,qq,qq') ∈ (loop_splits h e1 ++ loop_splits h e2).
 
   Lemma lc_disj_exit_to_exits_lsplits d : lc_disj_exit_lsplits_def d -> lc_disj_exits_lsplits_def d.
   Proof.
@@ -122,7 +167,7 @@ Module Disjoint.
         (Hneq : q1 <> q2 \/ j1 <> j2)
         (Hpath1 : TPath' ((p,i) :<: (q1,j1) :< t1))
         (Hpath2 : TPath' ((p,i) :<: (q2,j2) :< t2))
-    : exists qq qq' xl, (s,qq,qq',xl) ∈ splits p.
+    : exists qq qq', (s,qq,qq') ∈ splits p.
   Admitted.
 
   
